wip: lifting FL to LM

fairness/trace_helpers.v
@@ -96,7 +96,35 @@ Section FMTraceHelpers.
 
     Local Ltac gd t := generalize dependent t.
 
-    (* oℓ' ≠ Some ℓ *)
+    Definition label_kept_state_gen (Ps: St -> Prop) (Pstep: St -> option L -> St -> Prop) :=
+      forall st oℓ' st' (P1: Ps st) (PSTEP: Pstep st oℓ' st') (STEP: fmtrans _ st oℓ' st'), 
+        Ps st'.
+    
+    Lemma steps_keep_state_gen i (P: St -> Prop) Pstep j
+      (Pi: exists st, tr S!! i = Some st /\ P st)    
+      (* (P_KEPT: label_kept_state P Pl) *)
+      (P_KEPT: label_kept_state_gen P Pstep)
+      (NOρ: forall (k: nat) st1 oℓ' st2 (IKJ: i <= k < j), tr !! k = Some (st1, Some (oℓ', st2)) -> Pstep st1 oℓ' st2):
+      forall k st' (IKJ: i <= k <= j) (KTH: tr S!! k = Some st'), P st'.
+    Proof using VALID.
+      intros k st' [IK KJ]. apply Nat.le_sum in IK as [d ->]. gd st'. induction d.
+      { rewrite Nat.add_0_r. destruct Pi as (? & ? & ?). intros. congruence. }
+      intros st'' KTH. rewrite Nat.add_succ_r -Nat.add_1_r in KTH. 
+      pose proof (trace_has_len tr) as [len LEN]. 
+      forward eapply (proj2 (trace_lookup_dom_strong  _ _ LEN (i + d))) as [st' CUR].
+      { eapply state_lookup_dom; eauto. }
+      
+      destruct CUR as (oℓ' & st''_ & CUR).
+      pose proof CUR as (PREV & CUR' & STEP)%state_label_lookup. 
+      assert (st''_ = st'') as -> by congruence.
+      red in P_KEPT. eapply P_KEPT.
+      - apply IHd; [lia| eauto].
+      - eapply NOρ; eauto. lia. 
+      - eapply trace_valid_steps'; eauto. 
+    Qed.
+    
+
+    (* TODO: unify with general case *)
     Definition label_kept_state (Ps: St -> Prop) (Pl: option L -> Prop) :=
       forall st oℓ' st' (Pst: Ps st) (Poℓ: Pl oℓ') (STEP: fmtrans _ st oℓ' st'), 
         Ps st'.
@@ -125,6 +153,43 @@ Section FMTraceHelpers.
         apply state_label_lookup. eauto. 
     Qed.
     
+    (* (* TODO: rename *) *)
+    (* Lemma kept_state_fair_step' (ρ: L) (P: St -> Prop) *)
+    (*   (KEPT: label_kept_state P (other_step ρ)) *)
+    (*   (* (P_EN: forall st (Pst: P st), @role_enabled_model M ρ st) *) *)
+    (*   (FAIRρ: fair_model_trace ρ tr): *)
+    (*   forall i st (ITH: tr S!! i = Some st) (Pst: P st), *)
+    (*   exists j st', ClassicalFacts.Minimal (fun j => i <= j /\ tr L!! j = Some $ Some ρ \/ ¬ role_enabled_model ρ st') j /\ *)
+    (*              tr S!! j = Some st' /\ P st'. *)
+    (* Proof using VALID. *)
+    (*   intros.  *)
+    (*   apply fair_model_trace_defs_equiv, strong_fair_model_trace_alt_defs_equiv in FAIRρ.          *)
+    (*   red in FAIRρ. edestruct FAIRρ as [d [STEP MIN]]; [eauto| ..]. *)
+    (*   { apply P_EN. eauto. } *)
+    (*   clear FAIRρ.  *)
+
+    (*   pose proof (trace_has_len tr) as [len LEN]. *)
+    (*   assert (my_omega.NOmega.lt_nat_l (i + d) len) as DOMid. *)
+    (*   { destruct STEP as [(?&?&?) | STEP].  *)
+    (*     - eapply state_lookup_dom; eauto. *)
+    (*     - apply my_omega.NOmega.lt_lt_nat with (m := i + d + 1); [lia| ]. *)
+    (*       eapply label_lookup_dom; eauto. } *)
+    (*   pose proof (proj2 (state_lookup_dom _ _ LEN (i + d)) DOMid) as [st' IDTH]. *)
+      
+    (*   forward eapply steps_keep_state with (i := i) (j := i + d) (k := i + d) as NEXT_EN; eauto.  *)
+    (*   { intros. destruct IKJ as [[v ->]%Nat.le_sum KJ].  *)
+    (*     intros ->. enough (d <= v); [lia| ]. apply MIN. eauto. } *)
+    (*   { lia. } *)
+      
+    (*   destruct STEP as [(st'_ & ST' & DIS') | STEP]. *)
+    (*   { assert (st'_ = st') as -> by congruence.  *)
+    (*     destruct DIS'. apply P_EN. eauto. } *)
+    (*   exists (i + d), st'. split; eauto. *)
+    (*   red. split; [split; [lia| eauto]| ]. *)
+    (*   intros k [LE' STEP']. apply Nat.le_sum in LE' as [d' ->]. *)
+    (*   enough (d <= d'); [lia| ]. apply MIN. eauto. *)
+    (* Qed. *)
+
     (* TODO: rename *)
     Lemma kept_state_fair_step (ρ: L) (P: St -> Prop)
       (KEPT: label_kept_state P (other_step ρ))
