fairness/examples/ticketlock/fair_lock_lm.v
@@ -1,8 +1,37 @@
 From trillium.fairness.examples.ticketlock Require Import fair_lock.
-From trillium.fairness Require Import fuel lm_fair lm_fairness_preservation.
-From trillium.fairness.ext_models Require Import ext_models.
+From trillium.fairness.ext_models Require Import ext_models destutter_ext. 
 From iris.proofmode Require Import tactics.
 From stdpp Require Import base.
+From trillium.fairness Require Import  lm_fair_traces trace_helpers fuel lm_fair lm_fairness_preservation trace_lookup.
+
+
+(* TODO: move *)
+Lemma ev_rel_after `(FLP: FairLockPredicates M) `(EM: ExtModel M) tr ρ i atr
+  (* j atr *)
+  (EV_REL : eventual_release tr ρ i)
+  (AFTER: after i tr = Some atr)
+  :
+  (* eventual_release atr ρ (i - j). *)
+  eventual_release atr ρ 0.
+Proof.
+  red. intros ρ' k **. red in EV_REL.
+  specialize_full EV_REL.
+  { erewrite state_lookup_after in JTH; eauto. }
+  all: eauto.
+  { intros LE. specialize_full AFTER0; [lia| ]. destruct AFTER0 as [? RESTR].
+    split; auto.
+    intros. destruct BETWEEN as [[d ->]%Nat.le_sum LE2].  
+    eapply RESTR.
+    2: { erewrite state_lookup_after; eauto. }
+    lia. }
+  destruct EV_REL as (?&?&?&[d ->]%Nat.le_sum&?).
+  do 2 eexists. repeat split.
+  { erewrite state_lookup_after with (k := k + d); eauto.
+    by rewrite Nat.add_assoc. }
+  { lia. }
+  done.
+Qed. 
+
 
 
 Section FairLockLM.
@@ -82,13 +111,14 @@ Section FairLockLM.
   refine {| 
       can_lock_st := lift_prop1 can_lock_st;
       has_lock_st := lift_prop1 has_lock_st;
-      active_st := fun '(asG ρ) δ => 
-            ls_tmap (δ: fmstate LMF) !! (asG ρ) = Some {[ ρ ]} /\
-            (active_st ρ (ls_under δ) \/ default 0 (ls_fuel δ !! ρ) > 0);
+      (* active_st := fun '(asG ρ) δ =>  *)
+      (*       ls_tmap (δ: fmstate LMF) !! (asG ρ) = Some {[ ρ ]} /\ *)
+      (*       (active_st ρ (ls_under δ) \/ default 0 (ls_fuel δ !! ρ) > 0); *)
+      active_st := lift_prop1 active_st;
       is_unused := lift_prop1 is_unused;
       state_wf := wf_placeholder;
     |}.
-  intros [?] ?. solve_decision. 
+  (* intros [?] ?. solve_decision.  *)
   Defined.
 
   Let lift_prop2 (P: fmrole M -> fmstate M -> fmstate M -> Prop):
@@ -202,16 +232,261 @@ Section FairLockLM.
     red.
   Admitted. 
 
+  Let proj_ext (ι: @EI _ (FL_EM FLE_LMF)): @EI _ (FL_EM FLE) :=
+        match ι with
+        | flU (asG ρ) => flU ρ
+        | flL (asG ρ) => flL ρ
+        end. 
+    
+  Local Lemma PROJ_KEEP_EXT:
+    forall δ1 ι δ2, (@ETs _ (FL_EM FLE_LMF)) ι δ1 δ2 -> 
+                (@ETs _ (FL_EM FLE)) (proj_ext ι) (ls_under δ1) (ls_under δ2).
+  Proof. 
+    intros ? ι ? STEP. 
+    destruct ι as [[ρ]| [ρ]]; simpl in *; apply STEP.
+  Qed. 
+
+
+  
+  (* TODO: move, generalize *)
+  Lemma upto_state_lookup_unfold2 i δ
+    (lmtr: mtrace (@ext_model_FM LMF (@FL_EM LMF FLE_LMF)))
+    (mtr: trace M (option ext_role))
+    (UPTO: upto_stutter_eauxtr proj_ext lmtr mtr)
+    (ITH : lmtr S!! i = Some δ):
+    exists lmtr_i i' mtr_i',
+              after i lmtr = Some lmtr_i /\
+              after i' mtr = Some mtr_i' /\
+              upto_stutter ls_under (EUsls proj_ext) lmtr_i mtr_i' /\
+              mtr S!! i' = Some (ls_under δ).
+  Proof. 
+    pose proof ITH as (lmtr_i & AFTERi & TRi)%state_lookup_after'.
+    pose proof AFTERi as X. eapply upto_stutter_after' in X as (i' & mtr_i' & AFTERi' & UPTOi); eauto.
+    do 3 eexists. do 3 (try split; eauto).
+    rewrite -TRi.
+    erewrite state_lookup_after_0; eauto.
+    f_equal. eapply upto_stutter_trfirst; eauto.
+  Qed. 
+
+  (* TODO: move, generalize *)
+  Lemma upto_state_lookup_unfold1 i' st
+    (lmtr: mtrace (@ext_model_FM LMF (@FL_EM LMF FLE_LMF)))
+    (mtr: trace M (option ext_role))
+    (UPTO: upto_stutter_eauxtr proj_ext lmtr mtr)
+    (ITH : mtr S!! i' = Some st):
+    exists mtr_i' i lmtr_i,
+              after i lmtr = Some lmtr_i /\
+              after i' mtr = Some mtr_i' /\
+              upto_stutter ls_under (EUsls proj_ext) lmtr_i mtr_i' /\
+              st = ls_under (trfirst lmtr_i). 
+  Proof. 
+    pose proof ITH as (mtr_i' & AFTERi' & TRi')%state_lookup_after'.
+    pose proof AFTERi' as X. eapply upto_stutter_after in X as (i & lmtr_i & AFTERi & UPTOi); eauto.
+    do 3 eexists. do 3 (try split; eauto).
+    rewrite -TRi'.
+    eapply upto_stutter_trfirst; eauto.
+  Qed. 
 
   Lemma FL_LM_progress:
     @fair_lock_progress _ FLP_LMF (FL_EM FLE_LMF).
   Proof.
-    red. intros.
+    red. intros lmtr [ρ] i δ **.
     clear FAIR. 
     assert (∀ g: G,
-               fair_by_group (ELM_ALM LM_EM_EXT_KEEPS) g tr) as FAIR. 
+               fair_by_group (ELM_ALM LM_EM_EXT_KEEPS) g lmtr) as FAIR. 
     { admit. (* parametrize FairLock with the desired notion of fairness *) }
-    
+    pose proof (group_fairness_implies_role_fairness _ _ VALID FAIR) as FAIR'.
+    pose proof (can_destutter_eauxtr proj_ext _ VALID) as [mtr UPTO].
+    forward eapply destutter_ext.upto_preserves_validity as VALIDm; eauto. 
+    { apply PROJ_KEEP_EXT. }
+    forward eapply destutter_ext.upto_stutter_fairness as FAIRm; eauto.
+    { eapply ELM_ALM_afair_by_next; eauto. }
+    pose proof (@lock_progress _ _ _ FL) as PROGRESSm.    
+    red in PROGRESSm.
+
+    forward eapply upto_state_lookup_unfold2 as (lmtr_i & i' & mtr_i' & AFTERi & AFTERi' & UPTOi & ITH'); eauto. 
+      
+    specialize (PROGRESSm mtr_i' ρ 0 (ls_under δ)).
+    specialize_full PROGRESSm; eauto.
+    { eapply trace_valid_after; eauto. }
+    { admit. }
+    { do 2 red. intros. eapply fair_by_after; eauto. by apply FAIRm. }
+    { erewrite state_lookup_after; eauto. by rewrite Nat.add_0_r. }
+    { eapply ev_rel_after in EV_REL; eauto.
+      clear -EV_REL UPTOi.
+      rename mtr_i' into mtr. rename lmtr_i into lmtr. rename UPTOi into UPTO. 
+      red in EV_REL. 
+      red. intros.
+      forward eapply upto_state_lookup_unfold1 as (mtr_i' & i & lmtr_i & AFTERi & AFTERi' & UPTOi & ITH'); eauto.
+      
+      assert (∀ g : G, fair_by_group (ELM_ALM LM_EM_EXT_KEEPS) g lmtr_i) as FAIR. 
+      { admit. }
+      assert (lmtr S!! i = Some (trfirst lmtr_i)) as ITH.
+      { rewrite -(state_lookup_0 lmtr_i).
+        erewrite (state_lookup_after lmtr lmtr_i); eauto. }
+
+
+      assert (exists i' st', i <= i' /\
+                 lmtr S!! i' = Some st' /\ has_lock_st ρ' st' /\
+                          (* ¬ role_enabled_model ρ' st' /\ *)
+                          ρ' ∉ dom (ls_mapping st') /\
+                          ∀ (k : nat) (st' : fmstate ext_model_FM),
+           0 <= k <= i' - i
+           → lmtr_i S!! k = Some st'
+             → (λ δ : LiveState G M LSI,
+                  has_lock_st ρ' (ls_under δ)
+                  ∧ ¬ role_enabled_model ρ' (ls_under δ)) st').
+      { destruct (decide (ls_mapping (trfirst lmtr_i) !! ρ' = Some (asG ρ'))).
+        2: { exists i, (trfirst lmtr_i).
+             do 2 (split; [eauto| ]). split. 
+             { simpl. by rewrite -ITH'. }
+             split. 
+             { intros [? MAP]%elem_of_dom. apply n. rewrite MAP. 
+               admit. (* employ a corresponding LSI *) }
+             intros. assert (k = 0) as -> by lia.
+             erewrite state_lookup_after in H0; eauto.
+             rewrite Nat.add_0_r ITH in H0. inversion H0. subst. auto. }
+
+        assert (mtrace_valid lmtr_i) as VALIDi.
+        { admit. }
+
+        apply group_fairness_implies_step_or_unassign with (ρ := ρ') in FAIR.
+        2: done. 
+        apply fair_by_gen_equiv in FAIR.
+        red in FAIR. specialize (FAIR 0). specialize_full FAIR.
+        { erewrite state_lookup_after; eauto.
+          rewrite Nat.add_0_r ITH. simpl.
+          eapply elem_of_dom; eauto. }
+        simpl in FAIR. destruct FAIR as [m_ FAIR]. 
+        pattern m_ in FAIR. eapply min_prop_dec in FAIR as [m [FAIR MIN]].
+        2: { admit. }
+        destruct FAIR as (δ_m & step_m & MTH & FAIR).
+        red in FAIR.
+
+        Set Printing Coercions.
+        subst st'.
+
+        assert (
+               ∀ (k : nat) (st' : fmstate ext_model_FM),
+                   0 <= k <= m
+                   → lmtr_i S!! k = Some st'
+                     → (λ δ : LiveState G M LSI,
+                          has_lock_st ρ' (ls_under δ)
+                          ∧ ¬ role_enabled_model ρ' (ls_under δ)) st') as KEEP. 
+        { eapply steps_keep_state_gen. 
+          { eauto. }
+          { eexists. split; eauto. rewrite state_lookup_0. reflexivity. }
+          { (* TODO: move *)
+            Unshelve.
+            2: exact (fun δ1 oℓ δ2 => match oℓ with 
+                                   | Some (inl g) => lm_fair_traces.next_TS_role δ1 g δ2 ≠ Some ρ'
+                                   | oℓ => other_proj (asG ρ') oℓ
+                                   end). 
+            (* 2: exact (other_proj (asG ρ')).  *)
+            red. intros. simpl in STEP. inversion STEP; subst.
+            -
+              simpl in STEP0. unfold_LMF_trans STEP0.
+              + eapply step_keeps_lock_dis.
+                { split; [admit| ].
+                  apply P1. }
+                2: { simpl. left. simpl. apply STEP1. }                   
+                red. simpl. intros ->. congruence. 
+              + repeat apply proj2 in STEP1. congruence.
+            - destruct ι; simpl in REL; red in REL.
+              + destruct ρ0 as [ρ0]. 
+                eapply step_keeps_lock_dis.
+                { split; [admit| ].
+                  apply P1. }
+                2: { simpl. right. Unshelve. 2: exact (flU ρ0).
+                     apply REL. }
+                red. simpl.
+                intros ->. simpl in PSTEP. congruence.
+              + destruct ρ0 as [ρ0]. 
+                eapply step_keeps_lock_dis.
+                { split; [admit| ].
+                  apply P1. }
+                2: { simpl. right. Unshelve. 2: exact (flL ρ0).
+                     apply REL. }
+                red. simpl.
+                intros ->. simpl in PSTEP. congruence. }
+          { intros * [_ ?] KTH.
+            destruct oℓ'; [| done]. simpl. 
+            (* enough (m <= k); [lia| ]. apply MIN.      *)
+            (* apply trace_label_lookup_simpl' in KTH as (δ1&?&KTH). *)
+            pose proof KTH as STEP. eapply trace_valid_steps' in STEP; [| eauto].
+            simpl in STEP. 
+            destruct f as [| [ι]]. 
+            - intros EQ. specialize (MIN k). specialize_full MIN; [| lia].
+              do 2 eexists. split; [done| ].
+              red. right. simpl. red. simpl. do 3 eexists. repeat split; eauto.
+            - intros EQ. specialize (MIN k). specialize_full MIN; [| lia].
+              simpl in EQ. 
+              assert (ls_tmap st1 !! (asG ρ') = Some ∅) as NOρ.
+              { destruct ι; subst; inversion STEP; subst; simpl in REL; apply REL. }
+              do 2 eexists. split; [done| ].
+              left. intros (?& MAP)%elem_of_dom.
+              assert (x = asG ρ') as ->.
+              { admit. (* LSI *) }
+            eapply ls_mapping_tmap_corr in MAP as (?&?&?). 
+            set_solver. }
+          }
+
+          clear HAS_LOCK DIS.
+          pose proof (KEEP m) as KEEPm. specialize_full KEEPm. 
+          { split; [lia| reflexivity]. }
+          { eapply trace_state_lookup. apply MTH. }
+          destruct KEEPm as [HAS_LOCK DIS].
+
+        destruct FAIR as [UNMAP| STEP]. 
+        2: { simpl in STEP. red in STEP.
+             destruct STEP as (?&?&?&->&<-&STEP). 
+             apply next_TS_spec_pos in STEP.
+             simpl in STEP. 
+             destruct DIS. red. eapply fm_live_spec.
+             apply STEP. }
+
+        exists (i + m). eexists. split; [lia| ]. 
+        split; [| split]; [| | split| ..].
+          { apply trace_state_lookup in MTH.
+            erewrite state_lookup_after in MTH; [| eauto]. apply MTH. }
+          { eauto. }
+          { eauto. }
+          intros ??.
+          rewrite Nat.sub_add'. apply KEEP. }
+
+      clear HAS_LOCK DIS.      
+      destruct H as (m & δ_m & LEi & MTH & HAS_LOCK & UNMAP & BETWEEN). 
+      
+      specialize (EV_REL (asG ρ')). specialize_full EV_REL.
+      { apply MTH. }
+      { eauto. }
+      { intros [? STEP]%LM_live_roles_strong.
+        apply locale_trans_ex_role in STEP as [ρ'_ MAP].
+        assert (ρ'_ = ρ') as ->.
+        { admit. (* LSI *) }
+        by apply UNMAP, elem_of_dom. } 
+      { intros _. specialize (AFTER ltac:(lia)). destruct AFTER as [NEQ AFTER].
+        split; [congruence| ].
+        intros.
+        assert (k <= i \/ i <= k <= i + m) as [BEFORE | CUR] by lia. 
+        2: { intros LOCK2.
+             specialize (BETWEEN (k - i)). specialize_full BETWEEN.
+             { lia. }
+             { erewrite state_lookup_after; eauto.
+               rewrite -Nat.le_add_sub; eauto. lia. }
+             apply proj1 in BETWEEN. simpl in LOCK2.
+             eapply NEQ. eapply has_lock_st_excl; eauto. }
+        (* The prefix of mtr corresponding to this prefix of lmtr
+           doesn't have locks of ρ, according to AFTER.
+           Need to split trace more precisely, stating that both pre- and postfixes of traces a re related by upto_stutter
+         *)
+        admit. }
+
+      destruct EV_REL as (p & δ_p & PTH & LEm & ENp).
+      
+               
+      
+      
     
 
   Instance FL_LM: FairLock LMF FLP_LMF FLE_LMF.
